Hilbert10Experimental.lean
@@ -19,6 +19,7 @@ import Hilbert10Experimental.Instantiate
 import Hilbert10Experimental.Specialization
 import Hilbert10Experimental.CleanScratch
 import Hilbert10Experimental.CodeComp
+import Hilbert10Experimental.CodePair
 import Hilbert10Experimental.DiophToRE
 import Hilbert10Experimental.ExpDioph
 import Hilbert10Experimental.ExpDiophChoose
